@prefix cc: <http://creativecommons.org/ns#> .
@prefix dc: <http://purl.org/dc/elements/1.1/> .
@prefix dcterms: <http://purl.org/dc/terms/> .
@prefix error: <http://lodlaundromat.org/error/ontology/> .
@prefix foaf: <http://xmlns.com/foaf/0.1/> .
@prefix formats: <http://www.w3.org/ns/formats/> .
@prefix httpo: <http://lodlaundromat.org/http/ontology/> .
@prefix llm: <http://lodlaundromat.org/metrics/ontology/> .
@prefix llo: <http://lodlaundromat.org/ontology/> .
@prefix owl: <http://www.w3.org/2002/07/owl#> .
@prefix prov: <http://www.w3.org/ns/prov#> .
@prefix rdf: <http://www.w3.org/1999/02/22-rdf-syntax-ns#> .
@prefix rdfs: <http://www.w3.org/2000/01/rdf-schema#> .
@prefix vann: <http://purl.org/vocab/vann/> .
@prefix voaf: <http://purl.org/vocommons/voaf#> .
@prefix void: <http://rdfs.org/ns/void#> .
@prefix void-ext: <http://ldf.fi/void-ext#> .
@prefix xml: <http://www.w3.org/XML/1998/namespace> .
@prefix xsd: <http://www.w3.org/2001/XMLSchema#> .

<http://lodlaundromat.org/error/ontology/4xxHttpError> a owl:Class ;
    rdfs:label "4xx HTTP Error"@en-us ;
    rdfs:comment "An HTTP error in the 400-range."@en-us ;
    rdfs:subClassOf error:HttpError .

<http://lodlaundromat.org/error/ontology/5xxHttpError> a owl:Class ;
    rdfs:label "5xx HTTP Error"@en-us ;
    rdfs:comment "An HTTP error in the 500-range."@en-us ;
    rdfs:subClassOf error:HttpError .

error:CharacterEncodingError a owl:Class ;
    rdfs:label "character encoding error"@en-us ;
    rdfs:comment "An error due to the use of an illegitimate character code. The character code is stored under the error:object property."@en-us ;
    rdfs:subClassOf error:EncodingError .

error:DirectoryExistenceError a owl:Class ;
    rdfs:label "directory existence error"@en-us ;
    error:code "17"^^xsd:nonNegativeInteger ;
    error:message "File exists"^^xsd:string ;
    error:variableName "EXIST"^^xsd:string ;
    rdfs:comment "An error that occurs because a directory which is assumed to exist does not."@en-us ;
    rdfs:subClassOf error:ExistenceError .

error:DirectoryNotEmptyError a owl:Class ;
    rdfs:label "directory not empty"@en-us ;
    error:code "39"^^xsd:nonNegativeInteger ;
    error:message "Directory not empty"^^xsd:string ;
    error:variableName "ENOTEMPTY"^^xsd:string ;
    rdfs:comment "An error that occurs because a directory is assumed to be empty, but is not."@en-us ;
    rdfs:subClassOf error:ExistenceError .

error:FileExistenceError a owl:Class ;
    rdfs:label "file existence error"@en-us ;
    rdfs:comment "An error that occurs because a file which is assumed to exist does not."@en-us ;
    rdfs:subClassOf error:ExistenceError .

error:HttpUri a owl:Class ;
    rdfs:label "HTTP URI"@en-us ;
    rdfs:comment "A URI that uses the HTTP scheme."@en-us ;
    rdfs:subClassOf error:Object .

error:IsADirectoryError a owl:Class ;
    rdfs:label "source sink error"@en-us ;
    error:code "21"^^xsd:nonNegativeInteger ;
    error:message "Is a directory"^^xsd:string ;
    error:variableName "EISDIR"^^xsd:string ;
    rdfs:comment "???"@en-us ;
    rdfs:subClassOf error:ExistenceError .

error:MalformedUrl a owl:Class ;
    rdfs:label "malformed URL"@en-us ;
    rdfs:comment "An error that is thrown for a value which is expected to be a URL but does not conform to URL syntax."@en-us ;
    rdfs:subClassOf error:Error .

error:MissingTurtlePrefixDefinition a owl:Class ;
    rdfs:label "missing Turtle prefix definition"@en-us ;
    rdfs:comment "An error that occurs if a Turtle prefix is used but not defined."@en-us ;
    rdfs:subClassOf error:TurtleParserError .

error:PermissionError a owl:Class ;
    rdfs:label "permission error"@en-us ;
    rdfs:comment "An error that occurs because a specific action is not allowed to be performed w.r.t. a specific object that is of a given type."@en-us ;
    rdfs:subClassOf error:Error .

error:RedefinedRdfId a owl:Class ;
    rdfs:label "redefined RDF identifier"@en-us ;
    rdfs:comment "An error that is thrown whenever multiple definitions of the same resource occur in an RDF/XML document. This typically occurs whenever more than one rdf:Id statement occurs for the same resource."@en-us ;
    rdfs:subClassOf error:RdfxmlParserError .

error:SyntaxError a owl:Class ;
    rdfs:label "syntax position"@en-us ;
    rdfs:comment "A parser error that is due to the occurrence of an expression in the parsed data stream that does not conform to the expected grammar."@en-us ;
    rdfs:subClassOf error:ParserError .

error:XmlNameError a owl:Class ;
    rdfs:label "XML name error"@en-us ;
    rdfs:comment "The argument to rdf:ID is not an XML name."@en-us ;
    rdfs:subClassOf error:XmlParserError .

error:action a rdf:Property ;
    rdfs:label "action"@en-us ;
    rdfs:comment "The action to which the error is related."@en-us ;
    rdfs:domain error:Error ;
    rdfs:isDefinedBy error: ;
    rdfs:range error:Action .

error:character a rdf:Property ;
    rdfs:label "character"@en-us ;
    rdfs:comment "The character number of a stream position, indicating the number of characters that have preceded it."@en-us ;
    rdfs:domain error:StreamPosition ;
    rdfs:isDefinedBy error: ;
    rdfs:range xsd:integer .

error:code a rdf:Property ;
    rdfs:label "error code"@en-us ;
    rdfs:comment "Error code as used by the program in which the error occurs."@en-us ;
    rdfs:domain error:Error ;
    rdfs:isDefinedBy error: ;
    rdfs:range xsd:nonNegativeInteger .

error:column a rdf:Property ;
    rdfs:label "column"@en-us ;
    rdfs:comment "The column number of a stream position, indicating the number of characters that have preceded it since the last newline character or since the beginning of the stream."@en-us ;
    rdfs:domain error:StreamPosition ;
    rdfs:isDefinedBy error: ;
    rdfs:range xsd:integer .

error:connectionRefused a error:SocketError ;
    error:code "111"^^xsd:nonNegativeInteger ;
    error:message "Connection refused"^^xsd:string ;
    error:variableName "ECONNREFUSED"^^xsd:string ;
    rdfs:isDefinedBy error: .

error:connectionResetByPeer a error:ExistenceError,
        error:ReadError,
        error:SocketError ;
    error:code "104"^^xsd:nonNegativeInteger ;
    error:message "Connection reset by peer"^^xsd:string ;
    error:variableName "ECONNRESET"^^xsd:string ;
    rdfs:isDefinedBy error: .

error:connectionTimedOut a error:SocketError ;
    error:code "110"^^xsd:nonNegativeInteger ;
    error:message "Connection timed out"^^xsd:string ;
    error:variableName "ETIMEDOUT"^^xsd:string ;
    rdfs:isDefinedBy error: .

error:encodingError a error:WriteError ;
    rdfs:label "encoding error"@en-us ;
    rdfs:comment "Encoding cannot represent character."@en-us ;
    rdfs:isDefinedBy error: .

error:hostNotFound a error:SocketError ;
    rdfs:label "Host not found"@en-us ;
    rdfs:isDefinedBy error: .

error:illegalUtf8Continuation a error:ReadError ;
    rdfs:label "illegal UTF-8 continuation"@en-us ;
    rdfs:comment "Illegal UTF-8 continuation."@en-us ;
    rdfs:isDefinedBy error: .

error:illegalUtf8Start a error:ReadError ;
    rdfs:label "illegal UTF-8 start"@en-us ;
    rdfs:comment "Illegal UTF-8 start."@en-us ;
    rdfs:isDefinedBy error: .

error:invalidCentralDirectorySignature a error:ArchiveError ;
    error:code "25"^^xsd:nonNegativeInteger ;
    error:message "Invalid central directory signature."^^xsd:string ;
    rdfs:isDefinedBy error: .

error:isADirectory a error:ReadError ;
    rdfs:label "is a directory"@en-us ;
    error:code "21"^^xsd:nonNegativeInteger ;
    error:message "Is a directory"^^xsd:string ;
    error:variableName "EISDIR"^^xsd:string ;
    rdfs:comment "???"@en-us ;
    rdfs:isDefinedBy error: .

error:line a rdf:Property ;
    rdfs:label "column"@en-us ;
    rdfs:comment "The line number of a stream position, indicating the number of newline characters that have preceded it."@en-us ;
    rdfs:domain error:StreamPosition ;
    rdfs:isDefinedBy error: ;
    rdfs:range xsd:integer .

error:message a rdf:Property ;
    rdfs:label "error message"@en-us ;
    rdfs:comment "Error message for the human programmer."@en-us ;
    rdfs:domain error:Error ;
    rdfs:isDefinedBy error: ;
    rdfs:range xsd:string .

error:missingTypeKeywordInMtreeSpec a error:ArchiveError ;
    error:code "2"^^xsd:nonNegativeInteger ;
    error:message "Missing type keyword in mtree specification."^^xsd:string ;
    rdfs:isDefinedBy error: .

error:noData a error:SocketError ;
    rdfs:label "No data"@en-us ;
    error:code "61"^^xsd:nonNegativeInteger ;
    error:message "No data available"^^xsd:string ;
    error:variableName "ENODATA"^^xsd:string ;
    rdfs:isDefinedBy error: .

error:noRouteToHost a error:SocketError ;
    error:code "113"^^xsd:nonNegativeInteger ;
    error:message "No route to host"^^xsd:string ;
    error:variableName "EHOSTUNREACH"^^xsd:string ;
    rdfs:isDefinedBy error: .

error:notATypewriter a error:ReadError ;
    rdfs:label "not a typewriter"@en-us ;
    error:code "25"^^xsd:nonNegativeInteger ;
    error:message "Inappropriate ioctl for device"^^xsd:string ;
    error:variableName "ENOTTY"^^xsd:string ;
    rdfs:comment "Inappropriate input/output control for device."@en-us ;
    rdfs:isDefinedBy error: .

error:object a rdf:Property ;
    rdfs:label "object"@en-us ;
    rdfs:comment "The name of the object to which the error relates."@en-us ;
    rdfs:domain error:Error ;
    rdfs:isDefinedBy error: ;
    rdfs:range error:Object .

error:readTimeoutError a error:TimeoutError ;
    rdfs:label "read timeout error"@en-us ;
    rdfs:comment "Timeout occurs while reading"@en-us ;
    rdfs:isDefinedBy error: .

error:redirectAction a error:Action ;
    rdfs:label "redirect action"@en-us ;
    rdfs:comment "A rediraction action."@en-us ;
    rdfs:isDefinedBy error: .

error:sourceLine a rdf:Property ;
    rdfs:label "source line"@en-us ;
    rdfs:comment "The line number in the original source file for which a parser warning was thrown."@en-us ;
    rdfs:domain error:ParserError ;
    rdfs:isDefinedBy error: ;
    rdfs:range xsd:integer .

error:sslError a error:Error ;
    rdfs:label "SSL error"@en-us ;
    rdfs:comment "SSL error"@en-us ;
    rdfs:isDefinedBy error: .

error:streamPosition a rdf:Property ;
    rdfs:label "stream position"@en-us ;
    rdfs:comment "The stream position at which an error occurred."@en-us ;
    rdfs:domain error:Error ;
    rdfs:isDefinedBy error: ;
    rdfs:range error:StreamPosition .

error:tryAgain a error:SocketError ;
    rdfs:label "Try again"@en-us ;
    rdfs:isDefinedBy error: .

error:variableName a rdf:Property ;
    rdfs:label "variable name"@en-us ;
    rdfs:comment "The C variable name of the error as used in POSIX or in a Linux library or application."@en-us ;
    rdfs:domain error:Error ;
    rdfs:isDefinedBy error: ;
    rdfs:range xsd:string .

error:EncodingError a owl:Class ;
    rdfs:label "encoding error"@en-us ;
    rdfs:comment "An error due to the use of an illigitimate or unrecognized encoding."@en-us ;
    rdfs:subClassOf error:Error .

error:RdfxmlParserError a owl:Class ;
    rdfs:label "RDF/XML parser error"@en-us ;
    rdfs:comment "An that is emitted by an RDF/XML parser when it encounters data that does not conform to the RDF/XML grammar."@en-us ;
    rdfs:subClassOf error:RdfParserError,
        error:XmlParserError .

error:SgmlParserError a owl:Class ;
    rdfs:label "SGML parser error"@en-us ;
    rdfs:comment "A warning that is emitted by an SGML parser."@en-us ;
    rdfs:subClassOf error:ParserError .

error:TimeoutError a owl:Class ;
    rdfs:label "timeout error"@en-us ;
    rdfs:comment "An error that is thrown due to a timeout."@en-us ;
    rdfs:subClassOf error:Error .

error:TurtleParserError a owl:Class ;
    rdfs:label "XML parser error"@en-us ;
    rdfs:comment "A warning that is emitted by an XML parser."@en-us ;
    rdfs:subClassOf error:RdfParserError .

error:WriteError a owl:Class ;
    rdfs:label "write error"@en-us ;
    rdfs:comment "An error that occurs while writing data."@en-us ;
    rdfs:subClassOf error:IoError .

error:Action a owl:Class ;
    rdfs:label "action"@en-us ;
    rdfs:comment "An action performed by a computing device."@en-us ;
    rdfs:isDefinedBy error: .

error:ArchiveError a owl:Class ;
    rdfs:label "archive error"@en-us ;
    rdfs:comment "An error that occurs as part of an archive (un)packing process."@en-us ;
    rdfs:subClassOf error:Error .

error:HttpError a owl:Class ;
    rdfs:label "HTTP error"@en-us ;
    rdfs:comment "An error that is emitted as part of an HTTP reply."@en-us ;
    rdfs:subClassOf error:Error .

error:IoError a owl:Class ;
    rdfs:label "IO error"@en-us ;
    rdfs:comment "An error that was thrown due to an input and/or output issue."@en-us ;
    rdfs:subClassOf error:Error .

error:Object a owl:Class ;
    rdfs:label "object"@en-us ;
    rdfs:comment "An object that is related to an error."@en-us ;
    rdfs:isDefinedBy error: .

error:RdfParserError a owl:Class ;
    rdfs:label "RDF parser error"@en-us ;
    rdfs:comment "An error that is emitted by an RDF parser."@en-us ;
    rdfs:subClassOf error:ParserError .

error:XmlParserError a owl:Class ;
    rdfs:label "XML parser error"@en-us ;
    rdfs:comment "A warning that is emitted by an XML parser."@en-us ;
    rdfs:subClassOf error:SgmlParserError .

error:ParserError a owl:Class ;
    rdfs:label "parser error"@en-us ;
    rdfs:comment "An error that is emitted by a parser, indicating deviation from a defined grammar."@en-us ;
    rdfs:subClassOf error:Error .

error:StreamPosition a owl:Class ;
    rdfs:label "stream position"@en-us ;
    rdfs:comment "A position in a stream."@en-us ;
    rdfs:subClassOf error:Error .

error:ExistenceError a owl:Class ;
    rdfs:label "existence error"@en-us ;
    error:code "2"^^xsd:nonNegativeInteger ;
    error:message "No such file or directory"^^xsd:string ;
    error:variableName "ENOENT"^^xsd:string ;
    rdfs:comment "An error that occurs because a resource which is assumed to exist does not."@en-us ;
    rdfs:subClassOf error:Error .

error:ReadError a owl:Class ;
    rdfs:label "read error"@en-us ;
    rdfs:comment "An error that occurs while reading data."@en-us ;
    rdfs:subClassOf error:IoError .

error:SocketError a owl:Class ;
    rdfs:label "socket error"@en-us ;
    rdfs:comment "An error thrown because of a socket-related problem."@en-us ;
    rdfs:subClassOf error:Error .

error:Error a owl:Class ;
    rdfs:label "error"@en-us ;
    rdfs:comment "An recognized irregularity in program execution."@en-us ;
    rdfs:isDefinedBy error: .

error: a voaf:Vocabulary,
        owl:Ontology ;
    cc:license <http://creativecommons.org/licenses/by/3.0/> ;
    dc:creator [ a foaf:Person ;
            rdfs:isDefinedBy error: ;
            foaf:homepage <http://laurensrietveld.nl> ;
            foaf:name "Laurens Rietveld" ],
        [ a foaf:Person ;
            rdfs:isDefinedBy error: ;
            foaf:homepage <http://www.wouterbeek.com> ;
            foaf:name "Wouter Beek" ] ;
    dcterms:created "2014-09-24"^^xsd:date ;
    dcterms:description "Vocabulary for describing crawling errors, such as archive and http errors" ;
    dcterms:modified "2015-11-18"^^xsd:date ;
    dcterms:publisher "VU University Amsterdam" ;
    dcterms:title "Vocabulary for describing crawling errors" ;
    vann:preferredNamespacePrefix "error" ;
    vann:preferredNamespaceUri "http://lodlaundromat.org/error/ontology/" ;
    rdfs:isDefinedBy error: ;
    owl:versionInfo "1.0.1" ;
    foaf:homepage <http://lodlaundromat.org> .

