# baseURI: http://lodlaundromat.org/http/ontology/
# imports: http://lodlaundromat.org/resource/person

@prefix cc: <http://creativecommons.org/ns#> .
@prefix dc: <http://purl.org/dc/elements/1.1/> .
@prefix dcterms: <http://purl.org/dc/terms/> .
@prefix error: <http://lodlaundromat.org/error/ontology/> .
@prefix foaf: <http://xmlns.com/foaf/0.1/> .
@prefix formats: <http://www.w3.org/ns/formats/> .
@prefix http-w3c: <http://www.w3.org/2011/http#> .
@prefix httpo: <http://lodlaundromat.org/http/ontology/> .
@prefix llm: <http://lodlaundromat.org/metrics/ontology/> .
@prefix llo: <http://lodlaundromat.org/ontology/> .
@prefix owl: <http://www.w3.org/2002/07/owl#> .
@prefix person: <http://lodlaundromat.org/resource/person/> .
@prefix prov: <http://www.w3.org/ns/prov#> .
@prefix rdf: <http://www.w3.org/1999/02/22-rdf-syntax-ns#> .
@prefix rdfs: <http://www.w3.org/2000/01/rdf-schema#> .
@prefix vann: <http://purl.org/vocab/vann/> .
@prefix voaf: <http://purl.org/vocommons/voaf#> .
@prefix void: <http://rdfs.org/ns/void#> .
@prefix void-ext: <http://ldf.fi/void-ext#> .
@prefix xml: <http://www.w3.org/XML/1998/namespace> .
@prefix xsd: <http://www.w3.org/2001/XMLSchema#> .

httpo:
  rdf:type voaf:Vocabulary ;
  rdf:type owl:Ontology ;
  cc:license <http://creativecommons.org/licenses/by/3.0/> ;
  dc:creator person:laurens_rietveld ;
  dc:creator person:wouter_beek ;
  dc:creator person:rinke_hoekstra ;
  dcterms:created "2014-09-24"^^xsd:date ;
  dcterms:description "Vocabulary for describing http error codes" ;
  dcterms:modified "2015-11-18"^^xsd:date ;
  dcterms:publisher "VU University Amsterdam" ;
  dcterms:title "Vocabulary for describing http error codes" ;
  vann:preferredNamespacePrefix "httpo" ;
  vann:preferredNamespaceUri "http://lodlaundromat.org/http/ontology/" ;
  rdfs:isDefinedBy httpo: ;
  owl:imports <http://lodlaundromat.org/resource/person> ;
  owl:versionInfo "1.0.1" ;
  foaf:homepage <http://lodlaundromat.org> ;
.
<http://lodlaundromat.org/http/ontology/100>
  rdf:type <http://lodlaundromat.org/http/ontology/1xx> ;
  httpo:reasonPhrase "Continue"^^xsd:string ;
  httpo:statusCode 100 ;
  rdfs:comment "Indicates that the initial part of a request has been received and has not yet been rejected by the server. The server intends to send a final response after the request has been fully received and acted upon."@en-us ;
  rdfs:isDefinedBy httpo: ;
  rdfs:isDefinedBy <http://tools.ietf.org/html/rfc7231> ;
  rdfs:label "Continue"@en-us ;
.
<http://lodlaundromat.org/http/ontology/101>
  rdf:type <http://lodlaundromat.org/http/ontology/1xx> ;
  httpo:reasonPhrase "Switching Protocols"^^xsd:string ;
  httpo:statusCode 101 ;
  rdfs:comment "Indicates that the server understands and is willing to comply with the client's request, via the Upgrade header field for a change in the application protocol being used on this connection."@en-us ;
  rdfs:isDefinedBy httpo: ;
  rdfs:isDefinedBy <http://tools.ietf.org/html/rfc7231> ;
  rdfs:label "Switching Protocols"@en-us ;
.
<http://lodlaundromat.org/http/ontology/1xx>
  rdf:type owl:Class ;
  rdfs:comment "An HTTP status that is informational."@en-us ;
  rdfs:isDefinedBy httpo: ;
  rdfs:label "Informational"@en-us ;
  rdfs:subClassOf httpo:Status ;
.
<http://lodlaundromat.org/http/ontology/200>
  rdf:type <http://lodlaundromat.org/http/ontology/2xx> ;
  httpo:reasonPhrase "OK"^^xsd:string ;
  httpo:statusCode 200 ;
  rdfs:comment "Indicates that the request has succeeded."@en-us ;
  rdfs:isDefinedBy httpo: ;
  rdfs:isDefinedBy <http://tools.ietf.org/html/rfc7231> ;
  rdfs:label "OK"@en-us ;
.
<http://lodlaundromat.org/http/ontology/201>
  rdf:type <http://lodlaundromat.org/http/ontology/2xx> ;
  httpo:reasonPhrase "Created"^^xsd:string ;
  httpo:statusCode 201 ;
  rdfs:comment "Indicates that the request has been fulfilled and has resulted in one or more new resources being created."@en-us ;
  rdfs:isDefinedBy httpo: ;
  rdfs:isDefinedBy <http://tools.ietf.org/html/rfc7231> ;
  rdfs:label "Created"@en-us ;
.
<http://lodlaundromat.org/http/ontology/202>
  rdf:type <http://lodlaundromat.org/http/ontology/2xx> ;
  httpo:reasonPhrase "Accepted"^^xsd:string ;
  httpo:statusCode 202 ;
  rdfs:comment "Indicates that the request has been accepted for processing, but the processing has not been completed."@en-us ;
  rdfs:isDefinedBy httpo: ;
  rdfs:isDefinedBy <http://tools.ietf.org/html/rfc7231> ;
  rdfs:label "Accepted"@en-us ;
.
<http://lodlaundromat.org/http/ontology/203>
  rdf:type <http://lodlaundromat.org/http/ontology/2xx> ;
  httpo:reasonPhrase "Non-Authoritative Information"^^xsd:string ;
  httpo:statusCode 203 ;
  rdfs:comment "Indicates that the request was successful but the enclosed payload has been modified from that of the origin server's 200 (OK) response by a transforming proxy."@en-us ;
  rdfs:isDefinedBy httpo: ;
  rdfs:isDefinedBy <http://tools.ietf.org/html/rfc7231> ;
  rdfs:label "Non-Authoritative Information"@en-us ;
.
<http://lodlaundromat.org/http/ontology/204>
  rdf:type <http://lodlaundromat.org/http/ontology/2xx> ;
  httpo:reasonPhrase "No Content"^^xsd:string ;
  httpo:statusCode 204 ;
  rdfs:comment "Indicates that the server has successfully fulfilled the request and that there is no additional content to send in the response payload body."@en-us ;
  rdfs:isDefinedBy httpo: ;
  rdfs:isDefinedBy <http://tools.ietf.org/html/rfc7231> ;
  rdfs:label "No Content"@en-us ;
.
<http://lodlaundromat.org/http/ontology/205>
  rdf:type <http://lodlaundromat.org/http/ontology/2xx> ;
  httpo:reasonPhrase "Reset Content"^^xsd:string ;
  httpo:statusCode 205 ;
  rdfs:comment "Indicates that the server has fulfilled the request and desires that the user agent reset the \"document view\", which caused the request to be sent, to its original state as received from the origin server."@en-us ;
  rdfs:isDefinedBy httpo: ;
  rdfs:isDefinedBy <http://tools.ietf.org/html/rfc7231> ;
  rdfs:label "Reset Content"@en-us ;
.
<http://lodlaundromat.org/http/ontology/2xx>
  rdf:type owl:Class ;
  rdfs:comment "An HTTP status that is successful."@en-us ;
  rdfs:isDefinedBy httpo: ;
  rdfs:label "Successful"@en-us ;
  rdfs:subClassOf httpo:Status ;
.
<http://lodlaundromat.org/http/ontology/300>
  rdf:type <http://lodlaundromat.org/http/ontology/3xx> ;
  httpo:reasonPhrase "Multiple Choices"^^xsd:string ;
  httpo:statusCode 300 ;
  rdfs:comment "Indicates that the target resource has more than one representation, each with its own more specific identifier, and information about the alternatives is being provided so that the user (or user agent) can select a preferred representation by redirecting its request to one or more of those identifiers."@en-us ;
  rdfs:isDefinedBy httpo: ;
  rdfs:isDefinedBy <http://tools.ietf.org/html/rfc7231> ;
  rdfs:label "Multiple Choices"@en-us ;
.
<http://lodlaundromat.org/http/ontology/301>
  rdf:type <http://lodlaundromat.org/http/ontology/3xx> ;
  httpo:reasonPhrase "Moved Permanently"^^xsd:string ;
  httpo:statusCode 301 ;
  rdfs:comment "Indicates that the target resource has been assigned a new permanent URI and any future references to this resource ought to use one of the enclosed URIs."@en-us ;
  rdfs:isDefinedBy httpo: ;
  rdfs:isDefinedBy <http://tools.ietf.org/html/rfc7231> ;
  rdfs:label "Moved Permanently"@en-us ;
.
<http://lodlaundromat.org/http/ontology/302>
  rdf:type <http://lodlaundromat.org/http/ontology/3xx> ;
  httpo:reasonPhrase "Found"^^xsd:string ;
  httpo:statusCode 302 ;
  rdfs:comment "Indicates that the target resource resides temporarily under a different URI."@en-us ;
  rdfs:isDefinedBy httpo: ;
  rdfs:isDefinedBy <http://tools.ietf.org/html/rfc7231> ;
  rdfs:label "Found"@en-us ;
.
<http://lodlaundromat.org/http/ontology/303>
  rdf:type <http://lodlaundromat.org/http/ontology/3xx> ;
  httpo:reasonPhrase "See Other"^^xsd:string ;
  httpo:statusCode 303 ;
  rdfs:comment "Indicates that the server is redirecting the user agent to a different resource, as indicated by a URI in the Location header field, which is intended to provide an indirect response to the original request."@en-us ;
  rdfs:isDefinedBy httpo: ;
  rdfs:isDefinedBy <http://tools.ietf.org/html/rfc7231> ;
  rdfs:label "See Other"@en-us ;
.
<http://lodlaundromat.org/http/ontology/305>
  rdf:type <http://lodlaundromat.org/http/ontology/3xx> ;
  httpo:reasonPhrase "Use Proxy"^^xsd:string ;
  httpo:statusCode 305 ;
  rdfs:comment "The requested resource MUST be accessed through the proxy given by the Location field."@en-us ;
  rdfs:isDefinedBy httpo: ;
  rdfs:isDefinedBy <httpo://tools.ietf.org/html/rfc2616> ;
  rdfs:label "Use Proxy"@en-us ;
.
<http://lodlaundromat.org/http/ontology/306>
  rdf:type <http://lodlaundromat.org/http/ontology/3xx> ;
  httpo:reasonPhrase "Unused"^^xsd:string ;
  httpo:statusCode 306 ;
  rdfs:comment "Subsequent requests should use the specified proxy."@en-us ;
  rdfs:isDefinedBy httpo: ;
  rdfs:isDefinedBy <https://tools.ietf.org/html/draft-cohen-http-305-306-responses-00> ;
  rdfs:label "Unused"@en-us ;
.
<http://lodlaundromat.org/http/ontology/307>
  rdf:type <http://lodlaundromat.org/http/ontology/3xx> ;
  httpo:reasonPhrase "Temporary Redirect"^^xsd:string ;
  httpo:statusCode 307 ;
  rdfs:comment "Indicates that the target resource resides temporarily under a different URI and the user agent MUST NOT change the request method if it performs an automatic redirection to that URI."@en-us ;
  rdfs:isDefinedBy httpo: ;
  rdfs:isDefinedBy <http://tools.ietf.org/html/rfc7231> ;
  rdfs:label "Temporary Redirect"@en-us ;
.
<http://lodlaundromat.org/http/ontology/308>
  rdf:type <http://lodlaundromat.org/http/ontology/3xx> ;
  httpo:reasonPhrase "Permanent Redirect"^^xsd:string ;
  httpo:statusCode 308 ;
  rdfs:comment "The request, and all future requests should be repeated using another URI."@en-us ;
  rdfs:isDefinedBy httpo: ;
  rdfs:isDefinedBy <httpo://tools.ietf.org/html/rfc7238> ;
  rdfs:label "Permanent Redirect"@en-us ;
.
<http://lodlaundromat.org/http/ontology/3xx>
  rdf:type owl:Class ;
  rdfs:comment "An HTTP status that is a redirection."@en-us ;
  rdfs:isDefinedBy httpo: ;
  rdfs:label "Redirection"@en-us ;
  rdfs:subClassOf httpo:Status ;
.
<http://lodlaundromat.org/http/ontology/400>
  rdf:type <http://lodlaundromat.org/http/ontology/4xx> ;
  httpo:reasonPhrase "Bad Request"^^xsd:string ;
  httpo:statusCode 400 ;
  rdfs:comment "Indicates that the server cannot or will not process the request due to something that is perceived to be a client error."@en-us ;
  rdfs:isDefinedBy httpo: ;
  rdfs:isDefinedBy <http://tools.ietf.org/html/rfc7231> ;
  rdfs:label "Bad Request"@en-us ;
.
<http://lodlaundromat.org/http/ontology/402>
  rdf:type <http://lodlaundromat.org/http/ontology/4xx> ;
  httpo:reasonPhrase "Payment Required"^^xsd:string ;
  httpo:statusCode 402 ;
  rdfs:comment "Reserved for future use."@en-us ;
  rdfs:isDefinedBy httpo: ;
  rdfs:isDefinedBy <http://tools.ietf.org/html/rfc7231> ;
  rdfs:label "Payment Required"@en-us ;
.
<http://lodlaundromat.org/http/ontology/403>
  rdf:type <http://lodlaundromat.org/http/ontology/4xx> ;
  httpo:reasonPhrase "Forbidden"^^xsd:string ;
  httpo:statusCode 403 ;
  rdfs:comment "Indicates that the server understood the request but refuses to authorize it."@en-us ;
  rdfs:isDefinedBy httpo: ;
  rdfs:isDefinedBy <http://tools.ietf.org/html/rfc7231> ;
  rdfs:label "Forbidden"@en-us ;
.
<http://lodlaundromat.org/http/ontology/404>
  rdf:type <http://lodlaundromat.org/http/ontology/4xx> ;
  httpo:reasonPhrase "Not Found"^^xsd:string ;
  httpo:statusCode 404 ;
  rdfs:comment "Indicates that the origin server did not find a current representation for the target resource or is not willing to disclose that one exists."@en-us ;
  rdfs:isDefinedBy httpo: ;
  rdfs:isDefinedBy <http://tools.ietf.org/html/rfc7231> ;
  rdfs:label "Not Found"@en-us ;
.
<http://lodlaundromat.org/http/ontology/405>
  rdf:type <http://lodlaundromat.org/http/ontology/4xx> ;
  httpo:reasonPhrase "Method Not Allowed"^^xsd:string ;
  httpo:statusCode 405 ;
  rdfs:comment "Indicates that the method received in the request-line is known by the origin server but not supported by the target resource."@en-us ;
  rdfs:isDefinedBy httpo: ;
  rdfs:isDefinedBy <http://tools.ietf.org/html/rfc7231> ;
  rdfs:label "Method Not Allowed"@en-us ;
.
<http://lodlaundromat.org/http/ontology/406>
  rdf:type <http://lodlaundromat.org/http/ontology/4xx> ;
  httpo:reasonPhrase "Not Acceptable"^^xsd:string ;
  httpo:statusCode 406 ;
  rdfs:comment "Indicates that the target resource does not have a current representation that would be acceptable to the user agent, according to the proactive negotiation header fields received in the request, and the server is unwilling to supply a default representation."@en-us ;
  rdfs:isDefinedBy httpo: ;
  rdfs:isDefinedBy <http://tools.ietf.org/html/rfc7231> ;
  rdfs:label "Not Acceptable"@en-us ;
.
<http://lodlaundromat.org/http/ontology/408>
  rdf:type <http://lodlaundromat.org/http/ontology/4xx> ;
  httpo:reasonPhrase "Request Timeout"^^xsd:string ;
  httpo:statusCode 408 ;
  rdfs:comment "Indicates that the server did not receive a complete request message within the time that it was prepared to wait."@en-us ;
  rdfs:isDefinedBy httpo: ;
  rdfs:isDefinedBy <http://tools.ietf.org/html/rfc7231> ;
  rdfs:label "Request Timeout"@en-us ;
.
<http://lodlaundromat.org/http/ontology/409>
  rdf:type <http://lodlaundromat.org/http/ontology/4xx> ;
  httpo:reasonPhrase "Conflict"^^xsd:string ;
  httpo:statusCode 409 ;
  rdfs:comment "Indicates that the request could not be completed due to a conflict with the current state of the target resource."@en-us ;
  rdfs:isDefinedBy httpo: ;
  rdfs:isDefinedBy <http://tools.ietf.org/html/rfc7231> ;
  rdfs:label "Conflict"@en-us ;
.
<http://lodlaundromat.org/http/ontology/410>
  rdf:type <http://lodlaundromat.org/http/ontology/4xx> ;
  httpo:reasonPhrase "Gone"^^xsd:string ;
  httpo:statusCode 410 ;
  rdfs:comment "Indicates that access to the target resource is no longer available at the origin server and that this condition is likely to be permanent."@en-us ;
  rdfs:isDefinedBy httpo: ;
  rdfs:isDefinedBy <http://tools.ietf.org/html/rfc7231> ;
  rdfs:label "Gone"@en-us ;
.
<http://lodlaundromat.org/http/ontology/411>
  rdf:type <http://lodlaundromat.org/http/ontology/4xx> ;
  httpo:reasonPhrase "Length Required"^^xsd:string ;
  httpo:statusCode 411 ;
  rdfs:comment "Indicates that the server refuses to accept the request without a defined Content-Length."@en-us ;
  rdfs:isDefinedBy httpo: ;
  rdfs:isDefinedBy <http://tools.ietf.org/html/rfc7231> ;
  rdfs:label "Length Required"@en-us ;
.
<http://lodlaundromat.org/http/ontology/413>
  rdf:type <http://lodlaundromat.org/http/ontology/4xx> ;
  httpo:reasonPhrase "Payload Too Large"^^xsd:string ;
  httpo:statusCode 413 ;
  rdfs:comment "Indicates that the server is refusing to process a request because the request payload is larger than the server is willing or able to process."@en-us ;
  rdfs:isDefinedBy httpo: ;
  rdfs:isDefinedBy <http://tools.ietf.org/html/rfc7231> ;
  rdfs:label "Payload Too Large"@en-us ;
.
<http://lodlaundromat.org/http/ontology/414>
  rdf:type <http://lodlaundromat.org/http/ontology/4xx> ;
  httpo:reasonPhrase "URI Too Long"^^xsd:string ;
  httpo:statusCode 414 ;
  rdfs:comment "Indicates that the server is refusing to service the request because the request-target is longer than the server is willing to interpret."@en-us ;
  rdfs:isDefinedBy httpo: ;
  rdfs:isDefinedBy <http://tools.ietf.org/html/rfc7231> ;
  rdfs:label "URI Too Long"@en-us ;
.
<http://lodlaundromat.org/http/ontology/415>
  rdf:type <http://lodlaundromat.org/http/ontology/4xx> ;
  httpo:reasonPhrase "Unsupported Media Type"^^xsd:string ;
  httpo:statusCode 415 ;
  rdfs:comment "Indicates that the origin server is refusing to service the request because the payload is in a format not supported by this method on the target resource."@en-us ;
  rdfs:isDefinedBy httpo: ;
  rdfs:isDefinedBy <http://tools.ietf.org/html/rfc7231> ;
  rdfs:label "Unsupported Media Type"@en-us ;
.
<http://lodlaundromat.org/http/ontology/417>
  rdf:type <http://lodlaundromat.org/http/ontology/4xx> ;
  httpo:reasonPhrase "Expectation Failed"^^xsd:string ;
  httpo:statusCode 417 ;
  rdfs:comment "Indicates that the expectation given in the request's Expect header field could not be met by at least one of the inbound servers."@en-us ;
  rdfs:isDefinedBy httpo: ;
  rdfs:isDefinedBy <http://tools.ietf.org/html/rfc7231> ;
  rdfs:label "Expectation Failed"@en-us ;
.
<http://lodlaundromat.org/http/ontology/426>
  rdf:type <http://lodlaundromat.org/http/ontology/4xx> ;
  httpo:reasonPhrase "Upgrade Required"^^xsd:string ;
  httpo:statusCode 426 ;
  rdfs:comment "Indicates that the server refuses to perform the request using the current protocol but might be willing to do so after the client upgrades to a different protocol."@en-us ;
  rdfs:isDefinedBy httpo: ;
  rdfs:isDefinedBy <http://tools.ietf.org/html/rfc7231> ;
  rdfs:label "Upgrade Required"@en-us ;
.
<http://lodlaundromat.org/http/ontology/4xx>
  rdf:type owl:Class ;
  rdfs:comment "An HTTP status that is unsuccessful due to a client error."@en-us ;
  rdfs:isDefinedBy httpo: ;
  rdfs:label "Client Error"@en-us ;
  rdfs:subClassOf error:Exception ;
  rdfs:subClassOf httpo:Status ;
.
<http://lodlaundromat.org/http/ontology/501>
  rdf:type <http://lodlaundromat.org/http/ontology/5xx> ;
  httpo:reasonPhrase "Not Implemented"^^xsd:string ;
  httpo:statusCode 501 ;
  rdfs:comment "Indicates that the server does not support the functionality required to fulfill the request."@en-us ;
  rdfs:isDefinedBy httpo: ;
  rdfs:isDefinedBy <http://tools.ietf.org/html/rfc7231> ;
  rdfs:label "Not Implemented"@en-us ;
.
<http://lodlaundromat.org/http/ontology/502>
  rdf:type <http://lodlaundromat.org/http/ontology/5xx> ;
  httpo:reasonPhrase "Bad Gateway"^^xsd:string ;
  httpo:statusCode 502 ;
  rdfs:comment "Indicates that the server, while acting as a gateway or proxy, received an invalid response from an inbound server it accessed while attempting to fulfill the request."@en-us ;
  rdfs:isDefinedBy httpo: ;
  rdfs:isDefinedBy <http://tools.ietf.org/html/rfc7231> ;
  rdfs:label "Bad Gateway"@en-us ;
.
<http://lodlaundromat.org/http/ontology/503>
  rdf:type <http://lodlaundromat.org/http/ontology/5xx> ;
  httpo:reasonPhrase "Service Unavailable"^^xsd:string ;
  httpo:statusCode 503 ;
  rdfs:comment "Indicates that the server is currently unable to handle the request due to a temporary overload or scheduled maintenance, which will likely be alleviated after some delay."@en-us ;
  rdfs:isDefinedBy httpo: ;
  rdfs:isDefinedBy <http://tools.ietf.org/html/rfc7231> ;
  rdfs:label "Service Unavailable"@en-us ;
.
<http://lodlaundromat.org/http/ontology/504>
  rdf:type <http://lodlaundromat.org/http/ontology/5xx> ;
  httpo:reasonPhrase "Gateway Timeout"^^xsd:string ;
  httpo:statusCode 504 ;
  rdfs:comment "Indicates that the server, while acting as a gateway or proxy, did not receive a timely response from an upstream server it needed to access in order to complete the request."@en-us ;
  rdfs:isDefinedBy httpo: ;
  rdfs:isDefinedBy <http://tools.ietf.org/html/rfc7231> ;
  rdfs:label "Gateway Timeout"@en-us ;
.
<http://lodlaundromat.org/http/ontology/505>
  rdf:type <http://lodlaundromat.org/http/ontology/5xx> ;
  httpo:reasonPhrase "HTTP Version Not Supported"^^xsd:string ;
  httpo:statusCode 505 ;
  rdfs:comment "Indicates that the server does not support, or refuses to support, the major version of HTTP that was used in the request message."@en-us ;
  rdfs:isDefinedBy httpo: ;
  rdfs:isDefinedBy <http://tools.ietf.org/html/rfc7231> ;
  rdfs:label "HTTP Version Not Supported"@en-us ;
.
<http://lodlaundromat.org/http/ontology/5xx>
  rdf:type owl:Class ;
  rdfs:comment "An HTTP status that is unsuccessful due to a server error."@en-us ;
  rdfs:isDefinedBy httpo: ;
  rdfs:label "Server Error"@en-us ;
  rdfs:subClassOf error:Exception ;
  rdfs:subClassOf httpo:Status ;
.
httpo:Accept
  rdf:type httpo:ContentNegotiationHeader ;
  rdfs:isDefinedBy httpo: ;
  rdfs:label "Accept"@en-us ;
.
httpo:Accept-Charset
  rdf:type httpo:ContentNegotiationHeader ;
  rdfs:isDefinedBy httpo: ;
  rdfs:label "Accept-Charset"@en-us ;
.
httpo:Accept-Encoding
  rdf:type httpo:ContentNegotiationHeader ;
  rdfs:isDefinedBy httpo: ;
  rdfs:label "Accept-Encoding"@en-us ;
.
httpo:Accept-Language
  rdf:type httpo:ContentNegotiationHeader ;
  rdfs:isDefinedBy httpo: ;
  rdfs:label "Accept-Language"@en-us ;
.
httpo:CONNECT
  rdf:type owl:Class ;
  rdfs:comment "HTTP method for establishing a tunnel to the server identified by the target resource."@en-us ;
  rdfs:isDefinedBy httpo: ;
  rdfs:label "CONNECT"@en-us ;
  rdfs:subClassOf httpo:Method ;
.
httpo:Cache-Control
  rdf:type httpo:RequestHeader ;
  rdfs:isDefinedBy httpo: ;
  rdfs:label "Cache-Control"@en-us ;
.
httpo:CacheableMethod
  rdf:type owl:Class ;
  rdfs:comment "HTTP methods whose responses are allowed to be stored for future reuse."@en-us ;
  rdfs:isDefinedBy httpo: ;
  rdfs:label "HTTP cacheable method"@en-us ;
  rdfs:subClassOf httpo:Method ;
.
httpo:ConditionalHeader
  rdf:type owl:Class ;
  rdfs:comment "Allows a client to place a precondition on the state of the target resource, so that the action corresponding to the method semantics will not be applied if the precondition evaluates to false."@en-us ;
  rdfs:isDefinedBy httpo: ;
  rdfs:label "HTTP conditional header"@en-us ;
  rdfs:subClassOf httpo:Header ;
.
httpo:Content-Encoding
  rdf:type httpo:RepresentationHeader ;
  rdfs:isDefinedBy httpo: ;
  rdfs:label "Content-Encoding"@en-us ;
.
httpo:Content-Language
  rdf:type httpo:RepresentationHeader ;
  rdfs:isDefinedBy httpo: ;
  rdfs:label "Content-Language"@en-us ;
.
httpo:Content-Length
  rdf:type httpo:PayloadHeader ;
  rdfs:isDefinedBy httpo: ;
  rdfs:label "Content-Length"@en-us ;
.
httpo:Content-Location
  rdf:type httpo:RepresentationHeader ;
  rdfs:isDefinedBy httpo: ;
  rdfs:label "Content-Location"@en-us ;
.
httpo:Content-Range
  rdf:type httpo:PayloadHeader ;
  rdfs:isDefinedBy httpo: ;
  rdfs:label "Content-Range"@en-us ;
.
httpo:Content-Type
  rdf:type httpo:RepresentationHeader ;
  rdfs:isDefinedBy httpo: ;
  rdfs:label "Content-Type"@en-us ;
.
httpo:ContentNegotiationHeader
  rdf:type owl:Class ;
  rdfs:isDefinedBy httpo: ;
  rdfs:label "HTTP content negotiation header"@en-us ;
  rdfs:subClassOf httpo:Header ;
.
httpo:DELETE
  rdf:type owl:Class ;
  rdfs:comment "HTTP method for removing all current representations of the target resource."@en-us ;
  rdfs:isDefinedBy httpo: ;
  rdfs:label "DELETE"@en-us ;
  rdfs:subClassOf httpo:IdempotentMethod ;
  rdfs:subClassOf httpo:Method ;
.
httpo:Expect
  rdf:type httpo:RequestHeader ;
  rdfs:comment "Indication from a client that a certain set of behaviors (expectations) need to be supported by the server in order to properly handle the request."@en-us ;
  rdfs:isDefinedBy httpo: ;
  rdfs:label "Expect"@en-us ;
.
httpo:GET
  rdf:type owl:Class ;
  rdfs:comment "HTTP method for transfering a current representation of the target resource."@en-us ;
  rdfs:isDefinedBy httpo: ;
  rdfs:label "GET"@en-us ;
  rdfs:subClassOf httpo:CacheableMethod ;
  rdfs:subClassOf httpo:SafeMethod ;
.
httpo:HEAD
  rdf:type owl:Class ;
  rdfs:comment "HTTP method that only transfers the status line and header section of the target resource."@en-us ;
  rdfs:isDefinedBy httpo: ;
  rdfs:label "HEAD"@en-us ;
  rdfs:subClassOf httpo:CacheableMethod ;
  rdfs:subClassOf httpo:SafeMethod ;
.
httpo:Header
  rdf:type owl:Class ;
  rdfs:comment "An HTTP header."@en-us ;
  rdfs:isDefinedBy httpo: ;
  rdfs:label "HTTP header"@en-us ;
.
httpo:Host
  rdf:type httpo:RequestHeader ;
  rdfs:isDefinedBy httpo: ;
  rdfs:label "Host"@en-us ;
.
httpo:IdempotentMethod
  rdf:type owl:Class ;
  rdfs:comment "A request method whose intended effect on the server of multiple identical requests with that method is the same as the effect for a single such request."@en-us ;
  rdfs:isDefinedBy httpo: ;
  rdfs:label "HTTP idempotent method"@en-us ;
  rdfs:subClassOf httpo:Method ;
.
httpo:If-Match
  rdf:type httpo:ConditionalHeader ;
  rdfs:isDefinedBy httpo: ;
  rdfs:label "If-Match"@en-us ;
.
httpo:If-Modified-Since
  rdf:type httpo:ConditionalHeader ;
  rdfs:isDefinedBy httpo: ;
  rdfs:label "If-Modified-Since"@en-us ;
.
httpo:If-None-Match
  rdf:type httpo:ConditionalHeader ;
  rdfs:isDefinedBy httpo: ;
  rdfs:label "If-None-Match"@en-us ;
.
httpo:If-Range
  rdf:type httpo:ConditionalHeader ;
  rdfs:isDefinedBy httpo: ;
  rdfs:label "If-Range"@en-us ;
.
httpo:If-Unmodified-Since
  rdf:type httpo:ConditionalHeader ;
  rdfs:isDefinedBy httpo: ;
  rdfs:label "If-Unmodified-Since"@en-us ;
.
httpo:Max-Forwards
  rdf:type httpo:RequestHeader ;
  rdfs:comment "Mechanism for limiting the number of times a request is forwarded by proxies.Only supported for the OPTIONS and TRACE methods."@en-us ;
  rdfs:isDefinedBy httpo: ;
  rdfs:label "Max-Forwards"@en-us ;
.
httpo:Method
  rdf:type owl:Class ;
  rdfs:comment "Indicates the purpose for which the client has made a request and what is expected by the client as a successful result."@en-us ;
  rdfs:isDefinedBy httpo: ;
  rdfs:label "HTTP method"@en-us ;
.
httpo:OPTIONS
  rdf:type owl:Class ;
  rdfs:comment "HTTP method that describes the communication options for the target resource."@en-us ;
  rdfs:isDefinedBy httpo: ;
  rdfs:label "OPTIONS"@en-us ;
  rdfs:subClassOf httpo:SafeMethod ;
.
httpo:POST
  rdf:type owl:Class ;
  rdfs:comment "HTTP method that performs resource-specific processing on the request payload."@en-us ;
  rdfs:isDefinedBy httpo: ;
  rdfs:label "POST"@en-us ;
  rdfs:subClassOf httpo:CacheableMethod ;
.
httpo:PUT
  rdf:type owl:Class ;
  rdfs:comment "HTTP method that replaces all current representations of the target resource with the payload."@en-us ;
  rdfs:isDefinedBy httpo: ;
  rdfs:label "PUT"@en-us ;
  rdfs:subClassOf httpo:IdempotentMethod ;
.
httpo:PayloadHeader
  rdf:type owl:Class ;
  rdfs:comment "Header fields that specifically describe the payload, rather than the associated representation."@en-us ;
  rdfs:isDefinedBy httpo: ;
  rdfs:label "HTTP Payload Header"@en-us ;
  rdfs:subClassOf httpo:Header ;
.
httpo:Pragma
  rdf:type httpo:RequestHeader ;
  rdfs:isDefinedBy httpo: ;
  rdfs:label "Pragma"@en-us ;
.
httpo:Range
  rdf:type httpo:RequestHeader ;
  rdfs:isDefinedBy httpo: ;
  rdfs:label "Range"@en-us ;
.
httpo:RepresentationHeader
  rdf:type owl:Class ;
  rdfs:comment "Representation header fields provide metadata about the representation. When a message includes a payload body, the representation header fields describe how to interpret the representation data enclosed in the payload body. In a response to a HEAD request, the representation header fields describe the representation data that would have been enclosed in the payload body if the same request had been a GET."@en-us ;
  rdfs:isDefinedBy httpo: ;
  rdfs:label "HTTP representation header"@en-us ;
  rdfs:subClassOf httpo:Header ;
.
httpo:RequestHeader
  rdf:type owl:Class ;
  rdfs:comment "Request header fields provide metadata about the request context."@en-us ;
  rdfs:isDefinedBy httpo: ;
  rdfs:label "HTTP request header"@en-us ;
  rdfs:subClassOf httpo:Header ;
.
httpo:SafeMethod
  rdf:type owl:Class ;
  rdfs:comment "An HTTP method whose defined semantics is essentially read-only."@en-us ;
  rdfs:isDefinedBy httpo: ;
  rdfs:label "HTTP safe method"@en-us ;
  rdfs:subClassOf httpo:Method ;
.
httpo:Status
  rdf:type owl:Class ;
  rdfs:comment "A status that is returned by an HTTP server, indicating whether an HTTP request was handled successfully or not."@en-us ;
  rdfs:isDefinedBy httpo: ;
  rdfs:label "HTTP status"@en-us ;
  owl:equivalentClass http-w3c:StatusCode ;
.
httpo:TE
  rdf:type httpo:RequestHeader ;
  rdfs:isDefinedBy httpo: ;
  rdfs:label "TE"@en-us ;
.
httpo:TRACE
  rdf:type owl:Class ;
  rdfs:comment "HTTP method that performs a message loop-back test along the path to the target resource."@en-us ;
  rdfs:isDefinedBy httpo: ;
  rdfs:label "TRACE"@en-us ;
  rdfs:subClassOf httpo:SafeMethod ;
.
httpo:Trailer
  rdf:type httpo:PayloadHeader ;
  rdfs:isDefinedBy httpo: ;
  rdfs:label "Trailer"@en-us ;
.
httpo:Transfer-Encoding
  rdf:type httpo:PayloadHeader ;
  rdfs:isDefinedBy httpo: ;
  rdfs:label "Transfer-Encoding"@en-us ;
.
httpo:reasonPhrase
  rdf:type rdf:Property ;
  rdfs:comment "A natural language message describing an HTTP status."@en-us ;
  rdfs:domain httpo:Status ;
  rdfs:isDefinedBy httpo: ;
  rdfs:label "HTTP reason phrase"@en-us ;
  rdfs:range xsd:string ;
.
httpo:statusCode
  rdf:type rdf:Property ;
  rdfs:comment "The numeric indicator of an HTTP status."@en-us ;
  rdfs:domain httpo:Status ;
  rdfs:isDefinedBy httpo: ;
  rdfs:label "HTTP status code"@en-us ;
  rdfs:range xsd:integer ;
  owl:equivalentClass http-w3c:statusCodeNumber ;
.
