@prefix rdf: <http://www.w3.org/1999/02/22-rdf-syntax-ns#> .
@prefix bio: <http://bio2rdf.org/bio2rdf.dataset_vocabulary:> .
@prefix owl: <http://www.w3.org/2002/07/owl#> .
@prefix dcterms: <http://purl.org/dc/terms/> .
@prefix xsd: <http://www.w3.org/2001/XMLSchema#> .
@prefix vann: <http://purl.org/vocab/vann/> .
@prefix foaf: <http://xmlns.com/foaf/0.1/> .
@prefix dc: <http://purl.org/dc/elements/1.1/> .
@prefix void: <http://rdfs.org/ns/void#> .
@prefix rdfs: <http://www.w3.org/2000/01/rdf-schema#> .
@prefix formats: <http://www.w3.org/ns/formats/> .
@prefix void-ext: <http://ldf.fi/void-ext#> .
@prefix llm: <http://lodlaundromat.org/metrics/ontology/> .
@prefix llo: <http://lodlaundromat.org/ontology/> .
@prefix voaf: <http://purl.org/vocommons/voaf#> .
@prefix cc: <http://creativecommons.org/ns#> .
@prefix prov: <http://www.w3.org/ns/prov#>


<http://lodlaundromat.org/metrics/ontology/> 
	a owl:Ontology ;
	a voaf:Vocabulary;
	owl:versionInfo "1.0.1" ;
	owl:imports <http://rdfs.org/ns/void> ;
	owl:imports <http://ldf.fi/void-ext> ;
	owl:imports <http://bio2rdf.org/bio2rdf.dataset_vocabulary> ;
	dcterms:title "Collection (and extension) of several dataset metrics" ;
	dcterms:description "Collection (and extension) of several dataset metrics, including VoiD, VoiD-ext and Bio2RDF metrics" ;
	dcterms:modified "2015-05-20"^^xsd:date ;
	dcterms:created "2014-09-24"^^xsd:date ;
	foaf:homepage <http://lodlaundromat.org> ;
	vann:preferredNamespaceUri "http://lodlaundromat.org/metrics/ontology/";
    	vann:preferredNamespacePrefix "llm";
	dcterms:publisher "VU University Amsterdam" ;
	dc:creator 
		[a foaf:Person; foaf:name "Laurens Rietveld"; foaf:homepage <http://laurensrietveld.nl>] ,
		[a foaf:Person; foaf:name "Wouter Beek"; foaf:homepage <http://www.wouterbeek.com>] ;
	cc:license <http://creativecommons.org/licenses/by/3.0/> .


void:triples 
    rdfs:label "Number of triples";
    rdfs:comment "The total number of triples contained in the Dataset.".

void:classes
  rdfs:label "Number of distinct classes";
  rdfs:comment "The total number of distinct classes in a void:Dataset. In other words, the number of distinct resources occuring as objects of rdf:type triples in the dataset.".

void:properties 
    rdfs:label "Number of (distinct) properties";
    rdfs:comment "The total number of distinct properties in a void:Dataset. In other words, the number of distinct resources that occur in the predicate position of triples in the dataset.".



llm:definedClasses 
	a owl:DatatypeProperty;
  rdfs:label "Number of distinct defined classes";
  rdfs:comment "The total number of distinct defined classes in a void:Dataset. In other words, the number of distinct resources which have rdfs:Object or owl:Object as type.";
  rdfs:domain void:Dataset;
  rdfs:range xsd:long .



llm:definedProperties
	a owl:DatatypeProperty;
  rdfs:label "Number of distinct defined properties";
  rdfs:comment "The total number of distinct defined properties in a void:Dataset. In other words, the number of distinct resources which have rdfs:Property, owl:ObjectProperty, or owl:DatatypeProperty as type.";
  rdfs:domain void:Dataset;
  rdfs:range xsd:long .

void:entities
  rdfs:label "Number of distinct entities";
  rdfs:comment "The total number of distinct entities (IRIs) that are described in a void:Dataset.".

void:distinctObjects
    rdfs:label "Number of distinct objects";
    rdfs:comment "The total number of distinct objects in a void:Dataset. In other words, the number of distinct resources that occur in the object position of triples in the dataset. Literals are included in this count.".

void:distinctSubjects
    rdfs:label "Number of distinct subjects";
    rdfs:comment "The total number of distinct subjects in a void:Dataset. In other words, the number of distinct resources that occur in the subject position of triples in the dataset.".



void-ext:distinctRDFNodes
	rdfs:label "Distinct RDF nodes" ;
	rdfs:comment "The total number of distinct RDF nodes in a void:Dataset. In other words, the number of distinct literals, IRI references and blank nodes that occur in the subject, predicate or object position of triples in the dataset." .

llm:IRIs
	a owl:DatatypeProperty ;
	rdfs:label "Total number of IRI references" ;
	rdfs:comment "Total number of (non-distinct) IRI references in a void:Dataset. In other words, the number of distinct IRI references that occur in the subject, predicate or object position of triples in the dataset." ;
	rdfs:domain void:Dataset ;
	rdfs:range xsd:long .

void-ext:distinctIRIReferences
	rdfs:label "Distinct IRI references" ;
	rdfs:comment "The total number of distinct IRI references in a void:Dataset. In other words, the number of distinct IRI references that occur in the subject, predicate or object position of triples in the dataset." .

llm:blankNodes
	a owl:DatatypeProperty ;
	rdfs:label "Total number of blank nodes" ;
	rdfs:comment "The total number of (non-distinct) blank nodes in a void:Dataset. In other words, the number of distinct blank nodes that occur in the subject or object position of triples in the dataset." ;
	rdfs:domain void:Dataset ;
	rdfs:range xsd:long .

void-ext:distinctBlankNodes
	rdfs:label "Distinct blank nodes" ;
	rdfs:comment "The total number of distinct blank nodes in a void:Dataset. In other words, the number of distinct blank nodes that occur in the subject or object position of triples in the dataset." .

llm:literals
	a owl:DatatypeProperty ;
	rdfs:label "Total number of literals" ;
	rdfs:comment "The total number of (non-distinct) literals in a void:Dataset. In other words, the number of distinct literals that occur in the object position of triples in the dataset." ;
	rdfs:domain void:Dataset ;
	rdfs:range xsd:long .

void-ext:distinctLiterals
	rdfs:label "Distinct literals" ;
	rdfs:comment "The total number of distinct literals in a void:Dataset. In other words, the number of distinct literals that occur in the object position of triples in the dataset." .

void-ext:distinctIRIReferenceSubjects
	rdfs:label "Distinct IRIs in subject location" ;
	rdfs:comment "The total number of distinct IRIs as subjects in a void:Dataset. In other words, the number of distinct IRI references that occur in the subject position of triples in the dataset." .

void-ext:distinctBlankNodeSubjects
	rdfs:label "Distinct blank nodes in subject location" ;
	rdfs:comment "The total number of distinct blank nodes as subjects in a void:Dataset. In other words, the number of distinct blank nodes that occur in the subject position of triples in the dataset." .

void-ext:distinctIRIReferenceObjects
	rdfs:label "Distinct IRIs in object location" ;
	rdfs:comment "The total number of distinct IRIs as objects in a void:Dataset. In other words, the number of distinct IRI references that occur in the object position of triples in the dataset." .

void-ext:distinctBlankNodeObjects
	rdfs:label "Distinct blank nodes in object location" ;
	rdfs:comment "The total number of distinct blank nodes as objects in a void:Dataset. In other words, the number of distinct blank nodes that occur in the object position of triples in the dataset." .

void-ext:datatypes
	rdfs:label "Distinct literal datatypes" ;
	rdfs:comment "The total number of literal datatypes in a void:Dataset. In other words, the number of distinct datatypes that appear in any datatyped literal objects in the dataset." .

void-ext:languages
	rdfs:label "Distinct languages" ;
	rdfs:comment "The total number of literal languages in a void:Dataset. In other words, the number of distinct languages that appear in any language literal objects in the dataset." .

llm:IRILength
	a owl:ObjectProperty;
	rdfs:label "Statistics on the lengths of IRIs";
	rdfs:comment "Statistics on the lengths of IRIs, calculated on the non-distinct set of IRIs";
	rdfs:domain void:Dataset ;
	rdfs:range llm:descriptiveStatistics .

llm:subjectIRILength
	a owl:ObjectProperty;
	rdfs:label "Statistics on the lengths of subject IRIs";
	rdfs:comment "Statistics on the lengths of IRIs, calculated on the non-distinct set of IRIs occurring in the subject position";
	rdfs:domain void:Dataset ;
	rdfs:range llm:descriptiveStatistics .

llm:propertyIRILength
	a owl:ObjectProperty;
	rdfs:label "Statistics on the lengths of property IRIs";
	rdfs:comment "Statistics on the lengths of IRIs, calculated on the non-distinct set of IRIs occurring in the predicate position";
	rdfs:domain void:Dataset ;
	rdfs:range llm:descriptiveStatistics .

llm:objectIRILength
	a owl:ObjectProperty;
	rdfs:label "Statistics on the lengths of object IRIs";
	rdfs:comment "Statistics on the lengths of IRIs, calculated on the non-distinct set of IRIs occurring in the object position";
	rdfs:domain void:Dataset ;
	rdfs:range llm:descriptiveStatistics .

llm:literalLength
	a owl:ObjectProperty;
	rdfs:label "Statistics on the lengths of literals";
	rdfs:comment "Statistics on the lengths of a non-distinct set of literals. The length of the literal does not include language tags or datatypes";
	rdfs:domain void:Dataset ;
	rdfs:range llm:descriptiveStatistics .

llm:degree
	a owl:ObjectProperty;
	rdfs:label "Degree statistics";
	rdfs:comment "Statistics on the degrees of resources in this dataset.";
	rdfs:domain void:Dataset ;
	rdfs:range llm:descriptiveStatistics .
llm:outDegree
	a owl:ObjectProperty;
	rdfs:label "Out-degree statistics";
	rdfs:comment "Statistics on the out-degree of resources in this dataset, i.e. statistics on the out-links of resources, i.e. how often a resource occurs in a subject position";
	rdfs:domain void:Dataset ;
	rdfs:range llm:descriptiveStatistics .
	
llm:inDegree
	a owl:ObjectProperty;
	rdfs:label "In-degree statistics";
	rdfs:comment "Statistics on the in-degree of resources in this dataset, i.e. statistics on the incoming links of resources, i.e. how often a resource occurs in an object position";
	rdfs:domain void:Dataset ;
	rdfs:range llm:descriptiveStatistics .

llm:mean
	a owl:DatatypeProperty ; 
	rdfs:label "Mean";
	rdfs:comment "Mean";
	rdfs:domain llm:descriptiveStatistics;
	rdfs:range xsd:double .
	
llm:std
	a owl:DatatypeProperty ; 
	rdfs:label "Standard Deviation";
	rdfs:comment "Standard Deviation";
	rdfs:domain llm:descriptiveStatistics;
	rdfs:range xsd:double .

llm:median
	a owl:DatatypeProperty ; 
	rdfs:label "Median";
	rdfs:comment "Median";
	rdfs:domain llm:descriptiveStatistics;
	rdfs:range xsd:long .
	
llm:max
	a owl:DatatypeProperty ; 
	rdfs:label "Maximum";
	rdfs:comment "Maximum";
	rdfs:domain llm:descriptiveStatistics;
	rdfs:range xsd:long .

llm:min
	a owl:DatatypeProperty ; 
	rdfs:label "Minimum";
	rdfs:comment "Minimum";
	rdfs:domain llm:descriptiveStatistics;
	rdfs:range xsd:long .

llm:metrics
  a prov:Entity;
	a owl:ObjectProperty;
	rdfs:label "The dataset metrics";
	rdfs:comment "The dataset metrics for this document cleaned by the LOD Laundromat";
	rdfs:domain llo:DataDocument;
	rdfs:range void:Dataset.

llm:descriptiveStatistics
	a owl:Class;
	rdfs:label "Descriptive Statistics";
	rdfs:comment "A set of descriptive statistics, including the mean, standard deviation, median and min/max values".
	
