# baseURI: http://lodlaundromat.org/metrics/ontology/
# imports: http://ldf.fi/void-ext
# imports: http://lodlaundromat.org/ontology/
# imports: http://lodlaundromat.org/resource/person
# imports: http://rdfs.org/ns/void

@prefix : <http://lodlaundromat.org/metrics/ontology/> .
@prefix cc: <http://creativecommons.org/ns#> .
@prefix dc: <http://purl.org/dc/elements/1.1/> .
@prefix dcterms: <http://purl.org/dc/terms/> .
@prefix foaf: <http://xmlns.com/foaf/0.1/> .
@prefix formats: <http://www.w3.org/ns/formats/> .
@prefix httpo: <http://lodlaundromat.org/http/ontology/> .
@prefix llm: <http://lodlaundromat.org/metrics/ontology/> .
@prefix llo: <http://lodlaundromat.org/ontology/> .
@prefix owl: <http://www.w3.org/2002/07/owl#> .
@prefix person: <http://lodlaundromat.org/resource/person/> .
@prefix prov: <http://www.w3.org/ns/prov#> .
@prefix rdf: <http://www.w3.org/1999/02/22-rdf-syntax-ns#> .
@prefix rdfs: <http://www.w3.org/2000/01/rdf-schema#> .
@prefix vann: <http://purl.org/vocab/vann/> .
@prefix voaf: <http://purl.org/vocommons/voaf#> .
@prefix void: <http://rdfs.org/ns/void#> .
@prefix void-ext: <http://ldf.fi/void-ext#> .
@prefix xml: <http://www.w3.org/XML/1998/namespace> .
@prefix xsd: <http://www.w3.org/2001/XMLSchema#> .

void-ext:averageIRILength
  owl:propertyChainAxiom (
      llm:IRILength
      llm:mean
    ) ;
.
void-ext:averageLiteralLength
  owl:propertyChainAxiom (
      llm:literalLength
      llm:mean
    ) ;
.
void-ext:averageObjectIRILength
  owl:propertyChainAxiom (
      llm:objIRILength
      llm:mean
    ) ;
.
void-ext:averagePropertyIRILength
  owl:propertyChainAxiom (
      llm:predIRILength
      llm:mean
    ) ;
.
void-ext:averageSubjectIRILength
  owl:propertyChainAxiom (
      llm:subIRILength
      llm:mean
    ) ;
.
void-ext:distinctBlankNodes
  rdfs:subPropertyOf llm:blankNodes ;
.
void-ext:distinctLiterals
  rdfs:subPropertyOf llm:literals ;
.
llm:
  rdf:type voaf:Vocabulary ;
  rdf:type owl:Ontology ;
  cc:license <http://creativecommons.org/licenses/by/3.0/> ;
  dc:creator person:laurens_rietveld ;
  dc:creator person:rinke_hoekstra ;
  dc:creator person:wouter_beek ;
  dcterms:created "2014-09-24"^^xsd:date ;
  dcterms:description "Collection (and extension) of several dataset metrics, including VoiD, VoiD-ext and Bio2RDF metrics" ;
  dcterms:modified "2015-05-20"^^xsd:date ;
  dcterms:publisher "VU University Amsterdam" ;
  dcterms:title "Collection (and extension) of several dataset metrics" ;
  vann:preferredNamespacePrefix "llm" ;
  vann:preferredNamespaceUri "http://lodlaundromat.org/metrics/ontology/" ;
  voaf:classNumber 2 ;
  voaf:generalizes <http://ldf.fi/void-ext> ;
  voaf:propertyNumber 24 ;
  voaf:specializes <http://rdfs.org/ns/void> ;
  voaf:specializes <http://www.w3.org/ns/prov> ;
  voaf:usageInDataset <http://lodlaundromat.org> ;
  owl:imports <http://ldf.fi/void-ext> ;
  owl:imports llo: ;
  owl:imports <http://lodlaundromat.org/resource/person> ;
  owl:imports <http://rdfs.org/ns/void> ;
  owl:versionInfo "1.0.2" ;
  foaf:homepage <http://lodlaundromat.org> ;
.
llm:Dataset
  rdf:type owl:Class ;
  rdfs:comment "A dataset description"^^xsd:string ;
  rdfs:isDefinedBy llm: ;
  rdfs:label "Dataset"^^xsd:string ;
  rdfs:subClassOf void:Dataset ;
  rdfs:subClassOf prov:Entity ;
.
llm:DescriptiveStatistics
  rdf:type owl:Class ;
  rdfs:comment "A set of descriptive statistics, including the mean, standard deviation, median and min/max values" ;
  rdfs:isDefinedBy llm: ;
  rdfs:label "Descriptive Statistics" ;
.
llm:IRILength
  rdf:type owl:ObjectProperty ;
  rdfs:comment "Statistics on the lengths of IRIs, calculated on the non-distinct set of IRIs" ;
  rdfs:domain void:Dataset ;
  rdfs:isDefinedBy llm: ;
  rdfs:label "Statistics on the lengths of IRIs" ;
  rdfs:range llm:DescriptiveStatistics ;
  rdfs:subPropertyOf llm:statistics ;
.
llm:IRIs
  rdf:type owl:DatatypeProperty ;
  rdfs:comment "Total number of (non-distinct) IRI references in a void:Dataset. In other words, the number of distinct IRI references that occur in the subject, predicate or object position of triples in the dataset." ;
  rdfs:domain void:Dataset ;
  rdfs:isDefinedBy llm: ;
  rdfs:label "Total number of IRI references" ;
  rdfs:range xsd:long ;
  rdfs:subPropertyOf void:entities ;
.
llm:blankNodes
  rdf:type owl:DatatypeProperty ;
  rdfs:comment "The total number of (non-distinct) blank nodes in a void:Dataset. In other words, the number of distinct blank nodes that occur in the subject or object position of triples in the dataset." ;
  rdfs:domain void:Dataset ;
  rdfs:isDefinedBy llm: ;
  rdfs:label "Total number of blank nodes" ;
  rdfs:range xsd:long ;
.
llm:definedClasses
  rdf:type owl:DatatypeProperty ;
  rdfs:comment "The total number of distinct defined classes in a void:Dataset. In other words, the number of distinct resources which have rdfs:Object or owl:Object as type." ;
  rdfs:domain void:Dataset ;
  rdfs:isDefinedBy llm: ;
  rdfs:label "Number of distinct defined classes" ;
  rdfs:range xsd:long ;
  rdfs:subPropertyOf void:classes ;
.
llm:definedProperties
  rdf:type owl:DatatypeProperty ;
  rdfs:comment "The total number of distinct defined properties in a void:Dataset. In other words, the number of distinct resources which have rdfs:Property, owl:ObjectProperty, or owl:DatatypeProperty as type." ;
  rdfs:domain void:Dataset ;
  rdfs:isDefinedBy llm: ;
  rdfs:label "Number of distinct defined properties" ;
  rdfs:range xsd:long ;
  rdfs:subPropertyOf void:properties ;
.
llm:degree
  rdf:type owl:ObjectProperty ;
  rdfs:comment "Statistics on the degrees of resources in this dataset." ;
  rdfs:domain void:Dataset ;
  rdfs:isDefinedBy llm: ;
  rdfs:label "Degree statistics" ;
  rdfs:range llm:DescriptiveStatistics ;
  rdfs:subPropertyOf llm:statistics ;
.
llm:gitCommitId
  rdf:type owl:DatatypeProperty ;
  rdfs:comment "Commit ID belonging to a particular prov entity. Useful to refer to a GIT repository in any point in time" ;
  rdfs:domain prov:Entity ;
  rdfs:isDefinedBy llm: ;
  rdfs:label "Git Commit ID" ;
  rdfs:range xsd:string ;
.
llm:gitRepository
  rdf:type owl:ObjectProperty ;
  rdfs:comment "Repository URL belonging to a particular prov entity" ;
  rdfs:domain prov:Entity ;
  rdfs:isDefinedBy llm: ;
  rdfs:label "Git Repository URL" ;
.
llm:inDegree
  rdf:type owl:ObjectProperty ;
  rdfs:comment "Statistics on the in-degree of resources in this dataset, i.e. statistics on the incoming links of resources, i.e. how often a resource occurs in an object position" ;
  rdfs:domain void:Dataset ;
  rdfs:isDefinedBy llm: ;
  rdfs:label "In-degree statistics" ;
  rdfs:range llm:DescriptiveStatistics ;
  rdfs:subPropertyOf llm:statistics ;
.
llm:literalLength
  rdf:type owl:ObjectProperty ;
  rdfs:comment "Statistics on the lengths of a non-distinct set of literals. The length of the literal does not include language tags or datatypes" ;
  rdfs:domain void:Dataset ;
  rdfs:isDefinedBy llm: ;
  rdfs:label "Statistics on the lengths of literals" ;
  rdfs:range llm:DescriptiveStatistics ;
  rdfs:subPropertyOf llm:statistics ;
.
llm:literals
  rdf:type owl:DatatypeProperty ;
  rdfs:comment "The total number of (non-distinct) literals in a void:Dataset. In other words, the number of distinct literals that occur in the object position of triples in the dataset." ;
  rdfs:domain void:Dataset ;
  rdfs:isDefinedBy llm: ;
  rdfs:label "Total number of literals" ;
  rdfs:range xsd:long ;
.
llm:max
  rdf:type owl:DatatypeProperty ;
  rdfs:comment "Maximum" ;
  rdfs:domain llm:DescriptiveStatistics ;
  rdfs:isDefinedBy llm: ;
  rdfs:label "Maximum" ;
  rdfs:range xsd:long ;
  rdfs:subPropertyOf llm:value ;
.
llm:mean
  rdf:type owl:DatatypeProperty ;
  rdfs:comment "Mean" ;
  rdfs:domain llm:DescriptiveStatistics ;
  rdfs:isDefinedBy llm: ;
  rdfs:label "Mean" ;
  rdfs:range xsd:double ;
  rdfs:subPropertyOf llm:value ;
.
llm:median
  rdf:type owl:DatatypeProperty ;
  rdfs:comment "Median" ;
  rdfs:domain llm:DescriptiveStatistics ;
  rdfs:isDefinedBy llm: ;
  rdfs:label "Median" ;
  rdfs:range xsd:long ;
  rdfs:subPropertyOf llm:value ;
.
llm:metrics
  rdf:type owl:ObjectProperty ;
  rdfs:comment "The dataset metrics for this document cleaned by the LOD Laundromat" ;
  rdfs:domain llo:DataDocument ;
  rdfs:isDefinedBy llm: ;
  rdfs:label "The dataset metrics" ;
  rdfs:range void:Dataset ;
.
llm:metrics_of
  rdf:type owl:DatatypeProperty ;
  rdfs:domain llm:Dataset ;
  rdfs:isDefinedBy llm: ;
  owl:inverseOf llm:metrics ;
.
llm:min
  rdf:type owl:DatatypeProperty ;
  rdfs:comment "Minimum" ;
  rdfs:domain llm:DescriptiveStatistics ;
  rdfs:isDefinedBy llm: ;
  rdfs:label "Minimum" ;
  rdfs:range xsd:long ;
  rdfs:subPropertyOf llm:value ;
.
llm:objIRILength
  rdf:type owl:ObjectProperty ;
  rdfs:comment "Statistics on the lengths of IRIs, calculated on the non-distinct set of IRIs occurring in the object position" ;
  rdfs:domain void:Dataset ;
  rdfs:isDefinedBy llm: ;
  rdfs:label "Statistics on the lengths of object IRIs" ;
  rdfs:range llm:DescriptiveStatistics ;
  rdfs:subPropertyOf llm:statistics ;
.
llm:outDegree
  rdf:type owl:ObjectProperty ;
  rdfs:comment "Statistics on the out-degree of resources in this dataset, i.e. statistics on the out-links of resources, i.e. how often a resource occurs in a subject position" ;
  rdfs:domain void:Dataset ;
  rdfs:isDefinedBy llm: ;
  rdfs:label "Out-degree statistics" ;
  rdfs:range llm:DescriptiveStatistics ;
  rdfs:subPropertyOf llm:statistics ;
.
llm:predIRILength
  rdf:type owl:ObjectProperty ;
  rdfs:comment "Statistics on the lengths of IRIs, calculated on the non-distinct set of IRIs occurring in the predicate position" ;
  rdfs:domain void:Dataset ;
  rdfs:isDefinedBy llm: ;
  rdfs:label "Statistics on the lengths of predicate IRIs" ;
  rdfs:range llm:DescriptiveStatistics ;
  rdfs:subPropertyOf llm:statistics ;
.
llm:statistics
  rdf:type owl:ObjectProperty ;
  rdfs:domain llm:Dataset ;
  rdfs:isDefinedBy llm: ;
  rdfs:range llm:DescriptiveStatistics ;
.
llm:std
  rdf:type owl:DatatypeProperty ;
  rdfs:comment "Standard Deviation" ;
  rdfs:domain llm:DescriptiveStatistics ;
  rdfs:isDefinedBy llm: ;
  rdfs:label "Standard Deviation" ;
  rdfs:range xsd:double ;
  rdfs:subPropertyOf llm:value ;
.
llm:subIRILength
  rdf:type owl:ObjectProperty ;
  rdfs:comment "Statistics on the lengths of IRIs, calculated on the non-distinct set of IRIs occurring in the subject position" ;
  rdfs:domain void:Dataset ;
  rdfs:isDefinedBy llm: ;
  rdfs:label "Statistics on the lengths of subject IRIs" ;
  rdfs:range llm:DescriptiveStatistics ;
  rdfs:subPropertyOf llm:statistics ;
.
llm:value
  rdf:type owl:DatatypeProperty ;
  rdfs:domain llm:DescriptiveStatistics ;
.
void:triples
  owl:propertyChainAxiom (
      llm:metrics_of
      llo:triples
    ) ;
.
